design serializers

src/lean-serial.lean
@@ -1,15 +1,269 @@
 
+import tactic state
+import category.liftable
+import liftable
+
 universes u v
 
-structure serial (α : Type u) (β : Type v) :=
-  (encode : α → β)
-  (decode : β → option α)
-  (correctness : true) -- fill me up
+@[reducible]
+def put_m' (β : Type) (α : Type u) := α → state (ulift.{u} β) punit
+@[reducible]
+def get_m' (β : Type) := λ (α : Type u), state_t (ulift β) option α
 
-variables {α β γ φ : Type*}
+def serial_inverse {α} {β : Type u} (encode : put_m' α β) (decode : get_m' α β) : Prop :=
+∀ w, monad_state.lift (encode w) >> decode = pure w
 
-def compose : serial β γ → serial α β → serial α γ :=
-sorry -- fill me up
+structure medium :=
+  (rep : Type)
+  (encode_word : put_m' rep unsigned)
+  (decode_word : get_m' rep unsigned)
+  (inverse : serial_inverse encode_word decode_word)
+
+def medium.state (m : medium) := ulift m.rep
+
+@[reducible]
+def put_m (m : medium) := put_m' m.rep
+@[reducible]
+def get_m (m : medium) := get_m' m.rep
+
+instance (m : medium) : monad (get_m m) :=
+by apply_instance
+
+instance (m : medium) : is_lawful_monad (get_m m) :=
+by apply_instance
+
+instance (m : medium) : liftable1 (get_m.{u} m) (get_m.{v} m) :=
+by apply_instance
+
+class serial (α : Type u) :=
+  (encode : Π m : medium, put_m m α)
+  (decode : Π m : medium, get_m m α)
+  (correctness : ∀ m : medium, serial_inverse (encode m) (decode m))
+
+export serial (encode decode)
+
+structure serializer (α β : Type u) :=
+intl ::
+(encoder : Π m : medium, put_m m α)
+(decoder : Π m : medium, get_m m β)
+
+def valid_serializer {α} (x : serializer α α) :=
+∀ m : medium, serial_inverse
+      (serializer.encoder x m)
+      (serializer.decoder x m)
+
+def apply {α β} : α → (α → β) → β :=
+λ x (f : α → β), f x
+
+namespace serializer.seq
+
+variables {α i j : Type u}
+variables (x : serializer α (i → j))
+variables (y : serializer α i)
+
+def encoder (m : medium) := λ (k : α), x.encoder m k >> y.encoder m k
+def decoder (m : medium) := apply <$> y.decoder m <*> x.decoder m
+
+end serializer.seq
+
+instance {α : Type u} : applicative (serializer α) :=
+{ pure := λ i x, { encoder := λ _ _, return punit.star, decoder := λ k, pure x }
+, seq := λ i j x y,
+  { encoder := serializer.seq.encoder x y
+  , decoder := serializer.seq.decoder x y } }
+
+instance {α} : is_lawful_applicative (serializer α) :=
+begin
+  refine { .. }; dsimp; intros; casesm* serializer _ _;
+    simp [serializer.seq.encoder,serializer.seq.decoder];
+    split; ext,
+  all_goals
+  { simp [serializer.seq.encoder,serializer.seq.decoder,return,(>>),pure_bind,bind_pure,bind_assoc,pure_star,apply] with functor_norm },
+end
+
+def of_serializer {α} (s : serializer α α) (h : valid_serializer s) : serial α :=
+{ encode := s.encoder
+, decode := s.decoder
+, correctness := @h }
+
+def ser_field {α β} [serial β] (f : α → β) : serializer α β :=
+{ encoder := λ inst x, @encode _ _ inst (f x)
+, decoder := @decode _ _ }
+
+-- @[simp]
+-- lemma encoder_seq {γ α β : Type*} {ω} [medium ω]
+--   (x : serializer γ (α → β)) (y : serializer γ α) (w : γ) :
+--   (x <*> y).encoder ω w = (x.encoder ω w >> y.encoder ω w : state _ _) :=
+-- rfl
+
+-- @[simp]
+-- lemma encoder_map {γ α β : Type*} {ω} [medium ω]
+--   (x : α → β) (y : serializer γ α) (w : γ) :
+--   (x <$> y).encoder ω w = (y.encoder ω w : state _ _) :=
+-- by cases y; simp [functor.map,serializer.seq.encoder,(>>),pure_bind]
+
+-- @[simp]
+-- lemma encoder_field {α β : Type*} [serial β] {ω} [medium ω]
+--   (x : α → β) (w : α) :
+--   (ser_field x).encoder ω w = encode _ _ (x w) :=
+-- rfl
+
+open function
+
+variables {α β σ γ : Type u} {ω : Type}
+
+def there_and_back_again (m : medium)
+  (y : serializer γ α) (w : γ) : get_m m α :=
+monad_state.lift (y.encoder m w) >> y.decoder m
+
+@[simp]
+lemma decoder_pure (m : medium)
+  (x : α) :
+  (pure x : serializer γ α).decoder m = pure x := rfl
+
+@[simp]
+lemma decoder_seq (m : medium)
+  (f : serializer σ (α → β)) (x : serializer σ α) :
+  (f <*> x).decoder m = apply <$> x.decoder m <*> f.decoder m := rfl
+
+@[simp]
+lemma encoder_seq (m : medium)
+  (f : serializer σ $ α → β) (x : serializer σ α) (w : σ) :
+  (f <*> x).encoder m w = f.encoder m w >> x.encoder m w := rfl
+
+@[simp]
+lemma decoder_map (m : medium)
+  (f : α → β) (x : serializer σ α) :
+  (f <$> x).decoder m = f <$> x.decoder m :=
+by rw [← pure_seq_eq_map]; simp; simp [(∘),apply] with functor_norm
+
+@[simp]
+lemma encoder_map (m : medium)
+  (f : α → β) (x : serializer σ α) :
+  (f <$> x).encoder m = x.encoder m :=
+by { cases x, ext, simp! [functor.map,serializer.seq.encoder,(>>)] }
+
+@[simp]
+lemma encoder_field [serial β] (m : medium)
+  (f : α → β) :
+  (ser_field f).encoder m = λ w, encode _ m (f w) := rfl
+
+@[simp]
+lemma decoder_field [serial β] (m : medium)
+  (f : α → β) :
+  (ser_field f).decoder m = decode β m := rfl
+
+@[simp]
+lemma encode_decode_cancel [serial α] (m : medium)
+  (x : α) (f : α → get_m m β) :
+do { monad_state.lift (encode α m x),
+     decode α m >>= f } = f x :=
+by rw [← bind_assoc];
+     apply bind_eq_of_eq_pure;
+     [ apply serial.correctness,
+       refl ]
+
+@[simp]
+lemma lift_encoder_bind {β} (m : medium)
+  (encoder : put_m m α) (rest : state m.state β) (x : α) :
+  (monad_state.lift $ do { encoder x, rest } : get_m m _) =
+  do { monad_state.lift (encoder x), monad_state.lift rest }  :=
+is_lawful_monad_state.lift_bind _ _
+
+@[simp]
+lemma encode_decode_seq [serial α] (m : medium)
+  (x : serializer γ (α → β)) (y : γ → α) (w : γ) :
+  there_and_back_again m (x <*> ser_field y) w =
+  there_and_back_again m x w <*> pure (y w) :=
+by simp [there_and_back_again,apply] with functor_norm
+
+@[simp]
+lemma encode_decode_pure (m : medium) (x : β) (w : γ) :
+  there_and_back_again m (pure x) w =
+  pure x := rfl
+
+@[simp]
+lemma encode_decode_map [serial α] (m : medium)
+  (f : α → β) (y : γ → α) (w : γ) :
+  there_and_back_again m (f <$> ser_field y) w =
+  pure (f $ y w) :=
+by rw [← pure_seq_eq_map]; simp
+
+-- @[simp]
+-- lemma encode_decode_map {γ α β : Type*} {ω} (m : medium ω) (σ₀ : ω)
+--   (x : α → β) (y : serializer γ α) (w : γ) :
+--   there_and_back_again m (x <$> y) w (σ₀ : ω) =
+--   prod.map x id <$> there_and_back_again m y w σ₀ :=
+-- begin
+--   simp [there_and_back_again,serializer.seq.decoder,serializer.seq.encoder,(>>)] with functor_norm,
+--   congr' 1, ext z; cases z; simp [prod.map,const],
+-- end
+
+lemma valid_serializer_of_there_and_back_again
+      {α : Type*} (y : serializer α α) :
+  valid_serializer y ↔
+  ∀ (m : medium) (w : α), there_and_back_again m y w = pure w :=
+by { simp [valid_serializer,serial_inverse],
+     repeat { rw forall_congr, intro }, refl }
+
+-- lemma valid_serializer_seq {γ α β : Type*} {ω} (m : medium ω) (σ₀ : ω)
+--   (x : serializer γ (α → β)) (y : serializer γ α) (w : γ) :
+--   valid_serializer (x <*> y) := _
+open ulift
+
+def ulift.encode [serial α] (m : medium) (w : ulift.{v} α) : state (ulift $ medium.rep m) punit :=
+liftable1.up equiv.punit_equiv_punit (encode _ m (down w))
+
+def ulift.decode [serial α] (m : medium) : get_m m (ulift α) :=
+liftable1.down equiv.ulift (decode α m)
+
+instance [serial α] : serial (ulift α) :=
+{ encode := ulift.encode
+, decode := ulift.decode
+, correctness := by { introv _, simp [ulift.encode], rw monad_state_lift_liftable_up, simp [serial_inverse,monad_state_lift_liftable_up], rw monad_state_lift_liftable_up, apply medium.inverse } }
+
+instance : serial unsigned :=
+{ encode := λ γ inst w, @medium.encode_word γ inst ⟨w⟩
+, decode := λ γ inst, ulift.down <$> @medium.decode_word γ inst
+, correctness := by { introv w, simp, rw medium.inverse, refl } }
+
+structure point :=
+(x y : unsigned)
+
+section
+open tactic interactive interactive.types tactic.interactive (casesm trivial)
+
+meta def mk_serializer (s : parse texpr) : tactic unit :=
+do `(serial %%t) ← tactic.target,
+   refine ``(of_serializer %%s _),
+   `[simp [valid_serializer_of_there_and_back_again,serial_inverse], intros],
+   casesm none [to_pexpr t],
+   reflexivity <|> trivial
+
+run_cmd add_interactive [`mk_serializer]
+
+end
+
+instance : serial point :=
+by mk_serializer (point.mk <$> ser_field point.x <*> ser_field point.y)
+open ulift
+
+def prod.mk' {β : Type v} : ulift α → ulift β → (α × β) := _
+
+instance {β : Type v} [serial α] [serial β] : serial (α × β) :=
+by mk_serializer (prod.mk' <$> ser_field (up prod.fst) <*> ser_field (up prod.snd))
+
+#check bind_pure
+attribute [simp] serial.correctness
+
+variables {m : Type* → Type*} [monad m]
+
+variables {α β γ φ : Type u}
+
+def compose (x : serial β γ) (y : serial α β) : serial α γ :=
+{ encode := λ i z, x.encode (y.encode i _) z
+, decode := _ -- y.decode <=< x.decode
+, correctness := by intros; simp [monad.pipe] }
 
 local infixr ` ∘ ` := compose
 
@@ -17,14 +271,21 @@ variables (x : serial α β) (y : serial β γ) (z : serial γ φ)
 
 lemma compose_assoc :
   z ∘ (y ∘ x) = (z ∘ y) ∘ x :=
-sorry -- prove me!
+begin
+  casesm* serial _ _, dsimp [compose], congr' 1,
+  ext, simp [(<=<),bind_assoc],
+end
 
 def serial_unsigned : serial unsigned (list unsigned) :=
-sorry -- implementation please!
+{ encode := list.ret
+, decode := λ xs, list.nth xs 0
+, correctness := by intros; simp!; refl }
 
 def serial_pair (x : serial α (list unsigned)) (y : serial β (list unsigned)) :
   serial (α × β) (list unsigned) :=
-sorry -- implementation please!
+{ encode := λ i, x.encode i.1 ++ y.encode i.2
+, decode := _
+, correctness := _}
 
 def serial_sum (x : serial α (list unsigned)) (y : serial β (list unsigned)) :
   serial (α ⊕ β) (list unsigned) :=
