src/liftable.lean
@@ -1,0 +1,10 @@
+
+import category.liftable
+
+universes u v
+
+instance : liftable1 option.{u} option.{v} :=
+{ up := λ α β eq, @option.rec _ (λ _, option β) (@none β) (λ x, some $ eq x)
+, down := λ α β eq, @option.rec _ (λ _, option α) (@none α) (λ x, some $ eq.symm x)
+, up_down := by intros; cases x; simp
+, down_up := by intros; cases x; simp }
